tla_crash_safe_disk_refinement.dfy
@@ -6,28 +6,15 @@ import opened AppTypes
 import opened LogImpl
 import AbstractMap
 
-// Find a key in a log-representation map
-function {:opaque} ILogKey(log:seq<Datum>, k:int) : int
-{
-    if log==[]
-    then
-        AbstractMap.EmptyValue()
-    else if log[|log|-1].key == k
-    then
-        log[|log|-1].value
-    else
-        ILogKey(log[..|log|-1], k)
-}
-
 // Interpret a log sequence of Datums as a map
 function {:opaque} ILog(log:seq<Datum>) : imap<int, int>
 {
-    imap k | AbstractMap.InDomain(k) :: ILogKey(log, k)
+    imap k | AbstractMap.InDomain(k) :: EvalLog(log, k)
 }
 
 function {:opaque} DiskLogRecursive(k:Disk.Constants, s:Disk.Variables, len:nat) : seq<Datum>
-    requires len+1 <= k.size;
-    requires Disk.WF(k, s);
+    requires len+1 <= k.size
+    requires Disk.WF(k, s)
 {
     if len==0 
     then []
@@ -35,18 +22,30 @@ function {:opaque} DiskLogRecursive(k:Disk.Constants, s:Disk.Variables, len:nat)
 }
 
 // Interpret the disk as a Datum log
-function DiskLog(k:Constants, s:Variables) : seq<Datum>
-    requires DiskLogPlausible(k, s);
+function DiskLog(k:Disk.Constants, s:Disk.Variables) : seq<Datum>
+    requires DiskLogPlausible(k, s)
 {
-    var super := Disk.PeekF(k.disk, s.disk, 0);
-    DiskLogRecursive(k.disk, s.disk, super.value)
+    var super := Disk.PeekF(k, s, 0);
+    DiskLogRecursive(k, s, super.value)
+}
+
+lemma HowToMakeADiskLog(k:Disk.Constants, s:Disk.Variables, log:seq<Datum>)
+    requires DiskLogPlausible(k, s)
+    requires |log| <= Disk.PeekF(k, s, 0).value
+    requires forall i :: 0<=i<|log| ==> log[i] == Disk.PeekF(k, s, DiskLogAddr(i))
+    ensures DiskLogRecursive(k, s, |log|) == log
+{
+    reveal_DiskLogRecursive();
+    if log != [] {
+        HowToMakeADiskLog(k, s, log[..|log|-1]);
+    }
 }
 
 // Interpret the persistent system state (disk) as a map
 function IPersistent(k:Constants, s:Variables) : imap<int, int>
     requires Inv(k, s)
 {
-    ILog(DiskLog(k, s))
+    ILog(DiskLog(k.disk, s.disk))
 }
 
 // Interpret the ephemeral system state (memlog) as a map
@@ -60,7 +59,7 @@ function IEphemeral(k:Constants, s:Variables) : imap<int, int>
 
 // Refinement to an AbstractMap
 function I(k:Constants, s:Variables) : AbstractMap.Variables
-    requires Inv(k, s);
+    requires Inv(k, s)
 {
     AbstractMap.Variables(IEphemeral(k, s), IPersistent(k, s))
 }
@@ -71,29 +70,29 @@ function Ik(k:Constants) : AbstractMap.Constants
 }
 
 lemma InvImpliesRefinementInit(k:Constants, s:Variables)
-    requires Init(k, s);
-    ensures AbstractMap.Init(Ik(k), I(k, s));
+    requires Init(k, s)
+    ensures AbstractMap.Init(Ik(k), I(k, s))
 {
     reveal_ILog();
-    reveal_ILogKey();
+    reveal_FindIndexInLog();
     assert IEphemeral(k, s) == AbstractMap.EmptyMap();  // OBSERVE
     reveal_DiskLogRecursive();
 } 
 
 lemma InvImpliesWF(k:Constants, s:Variables)
-    requires Inv(k, s);
-    ensures AbstractMap.WF(I(k, s));
+    requires Inv(k, s)
+    ensures AbstractMap.WF(I(k, s))
 {
     reveal_ILog();
-    reveal_ILogKey();
+    reveal_FindIndexInLog();
 }
 
 lemma InvImpliesRefinementNext(k:Constants, s:Variables, s':Variables)
-    requires Next(k, s, s');
-    requires Inv(k, s);
-    ensures AbstractMap.WF(I(k, s));
-    ensures AbstractMap.WF(I(k, s'));
-    ensures AbstractMap.Next(Ik(k), I(k, s), I(k, s'));
+    requires Next(k, s, s')
+    requires Inv(k, s)
+    ensures AbstractMap.WF(I(k, s))
+    ensures AbstractMap.WF(I(k, s'))
+    ensures AbstractMap.Next(Ik(k), I(k, s), I(k, s'))
 {
     var Ik := Ik(k);
     var Is := I(k, s);
@@ -107,18 +106,6 @@ lemma InvImpliesRefinementNext(k:Constants, s:Variables, s':Variables)
 
     match step {
         case CrashAndRecover => {
-//            assert !s'.mode.Running?;
-//            assert Disk.Idle(k.disk, s.disk, s'.disk);
-//            assert DiskLog(k, s) == DiskLog(k, s');
-//            calc {
-//                Is'.ephemeral;
-//                IEphemeral(k, s');
-//                //if s'.mode.Running? then ILog(s'.memlog) else IPersistent(k, s');
-//                IPersistent(k, s');
-//                IPersistent(k, s);
-//                Is.persistent;
-//            }
-//            assert Is'.persistent == Is.persistent;
             assert AbstractMap.NextStep(Ik, Is, Is', AbstractMap.SpontaneousCrash);
         }
         case ReadSuperblock => {
@@ -128,12 +115,19 @@ lemma InvImpliesRefinementNext(k:Constants, s:Variables, s':Variables)
             assert AbstractMap.NextStep(Ik, Is, Is', AbstractMap.Stutter());
         }
         case TerminateScan => {
+            HowToMakeADiskLog(k.disk, s.disk, s.memlog);
             assert AbstractMap.NextStep(Ik, Is, Is', AbstractMap.Stutter());
         }
         case Append(datum) => {
             assert AbstractMap.NextStep(Ik, Is, Is', AbstractMap.Write(datum));
         }
         case Query(datum) => {
+            calc {
+                datum.value;
+                EvalLog(s.memlog, datum.key).value;
+                IEphemeral(k, s)[datum.key];
+            }
+            assert Is' == Is;
             assert AbstractMap.NextStep(Ik, Is, Is', AbstractMap.Query(datum));
         }
         case PushLogData => {
